SporkProofs/ParReduce.lean
@@ -1,40 +1,47 @@
 import SporkProofs.Syntax
 import SporkProofs.Notation
+import SporkProofs.WFSyntax
 
-def parSSA (f g : FuncIdx): Func :=
+def parSSAexample: Program :=
+  let f := 0
+  let g := 1
+  .mk [
+    func ()
+    func (
+      block start() {SPORK (goto body(), goto spwn())},
+      block body() {CALL f() ⊳ goto cont()},
+      block cont(x) {SPOIN (goto unpr(x), goto prom(x))},
+      block unpr(x) {CALL g() ⊳ goto ret(x)},
+      block prom(x, y) {GOTO ret(x,y)},
+      block ret(x, y) {RETURN(x, y)},
+      block spwn() {CALL g() ⊳ goto exit()},
+      block exit(y) {RETURN(y)}
+    )]
+
+
+def redSSA (c f red : FuncIdx) : Func :=
   func (
-    block start() {SPORK (goto body(), g())},
-    block body() sporks (1) {CALL f() ⊳ goto cont()},
-    block cont(x) sporks (1) {SPOIN (goto unpr(x), goto prom(x))},
-    block unpr(x) {CALL g() ⊳ goto ret(x)},
-    block prom(x, y) {GOTO ret(x,y)},
-    block ret(x, y) {RETURN(x, y)}
-  )
-
-def redSSA (c f red split : FuncIdx) : Func × Func :=
-  (func (
-     block start(z,a,i,j) {GOTO guard(z,i,j,a)},
-     block guard(z,i,j,a) {b ← i >= j, IF b THEN goto done(a) ELSE goto iter(z,i,j,a)},
-     block done(a) {RETURN(a)},
-     block iter(z,i,j,a) {SPORK (goto body(z,i,j,a), split(z,i,j,a))},
-     block body(z,i,j,a) sporks (1) {CALL f(i) ⊳ goto accum(z,i,j,a)},
-     block accum(z,i,j,a,a₁) sporks (1) {CALL c(a,a₁) ⊳ goto cont(z,i,j)},
-     block cont(z,i,j,a) sporks (1) {SPOIN (goto next(z,i,j,a), goto brk(a))},
-     block next(z,i,j,a) {i₁ ← i + 1, GOTO guard(z,i₁,j,a)},
-     block brk(a,a₁) {CALL c(a,a₁) ⊳ goto done()}
-   ),
-   func (
-     block spwn(z,a,i,j) {i₁ ← i + 1, k ← i₁ + j, m ← k / 2, SPORK (goto left(z,i₁,m,j), red(z,z,m,j))},
-     block left(z,i,m,j) sporks (1) {CALL red(z,z,i,m) ⊳ goto middle(z,m,j)},
-     block middle(z,m,j,a) sporks (1) {SPOIN(goto leftover(z,m,j,a), goto merge(a))},
-     block leftover(z,m,j,a) {CALL red(z,a,m,j) ⊳ goto exit()},
-     block merge(a,a₁) {CALL c(a,a₁) ⊳ goto exit()},
-     block exit(a) {RETURN(a)}
-   ))  
+    block start(z,a,i,j) {GOTO guard(z,i,j,a)},
+    block guard(z,i,j,a) {b ← i >= j, IF b THEN goto done(a) ELSE goto iter(z,i,j,a)},
+    block done(a) {RETURN(a)},
+    block iter(z,i,j,a) {SPORK (goto body(z,i,j,a), goto split(z,i,j,a))},
+    block body(z,i,j,a) {CALL f(i) ⊳ goto accum(z,i,j,a)},
+    block accum(z,i,j,a,a₁) {CALL c(a,a₁) ⊳ goto cont(z,i,j)},
+    block cont(z,i,j,a) {SPOIN (goto next(z,i,j,a), goto brk(a))},
+    block next(z,i,j,a) {i₁ ← i + 1, GOTO guard(z,i₁,j,a)},
+    block brk(a,a₁) {CALL c(a,a₁) ⊳ goto done()},
+    block split(z,i,j,a) {i₁ ← i + 1, k ← i₁ + j, m ← k / 2, SPORK (goto left(z,i₁,m,j), goto right(z,m,j))},
+    block left(z,i,m,j) {CALL red(z,z,i,m) ⊳ goto middle(z,m,j)},
+    block middle(z,m,j,a) {SPOIN(goto leftover(z,m,j,a), goto merge(a))},
+    block leftover(z,m,j,a) {CALL red(z,a,m,j) ⊳ goto exit()},
+    block merge(a,a₁) {CALL c(a,a₁) ⊳ goto exit()},
+    block exit(a) {RETURN(a)},
+    block right(z,m,j) {CALL red(z,z,m,j) ⊳ goto exit()}
+   )
 
 theorem parSSAWF : (parSSA 0 1).WF [FuncSig.mk 0 1, FuncSig.mk 0 1] :=
   by trivial
 theorem redSSAWF :
     let fsigs := [FuncSig.mk 2 1, FuncSig.mk 1 1, FuncSig.mk 4 1, FuncSig.mk 4 1]
-    (redSSA 0 1 2 3).fst.WF fsigs ∧ (redSSA 0 1 2 3).snd.WF fsigs :=
+    (redSSA 0 1 2).WF fsigs
   by trivial
