SporkProofs/Syntax.lean
@@ -1,7 +1,7 @@
-import SporkProofs.IVec
-import SporkProofs.HeadIs
-
 abbrev Val := Int
+
+abbrev Scope := Nat
+abbrev Params := Nat
 
 inductive Var where
   | mk (v : Nat)
@@ -35,39 +35,39 @@ inductive Code where
   | ite (cond : Atom) (bthen : Cont) (belse : Cont)
   | call (f : FuncIdx) (args : List Var) (bret : Cont)
   | retn (args : List Var)
-  | spork (n : Nat) (bbody : Cont) (bspwn : Cont)
+  | spork (bbody : Cont) (bspwn : Cont)
   | spoin (bunpr : Cont) (bprom : Cont)
-  | join (bsync : Cont)
-  | exit (args : List Var)
+  -- | join (bsync : Cont)
+  -- | exit (args : List Var)
 
---abbrev SporkSig := List Nat
 -- Obligation to return, exit, spoin, or join
-inductive Oblg where
-  | retn (n : Nat)
-  | exit (n : Nat)
-  | spoin (σ : Oblg) (n : Nat)
-  | join (σ : Oblg) (n : Nat)
+-- inductive Oblg where
+--   | retn (n : Nat)
+--   | exit (n : Nat)
+--   | spoin (σ : Oblg) (n : Nat)
+--   | join (σ : Oblg) (n : Nat)
 
--- block with `arity` args and nested under `sporks`
+-- block with a local scope Γ which must return r values and obligated to spoin σ
 inductive BlockSig where
-  | mk (arity : Nat) (oblg : Oblg)
+  | mk (Γ : Nat) (r : Nat) (σ : List Nat)
 
 inductive Block where
   | mk (bsig : BlockSig) (code : Code)
 
 inductive FuncSig where
-  | mk (arity : Nat) (ret : Nat)
+  | mk (params : Params) (ret : Nat)
 
 inductive Func where
   | mk (fsig : FuncSig) (blocks : List Block)
 
 inductive Program where
-  | mk (funs : List Func) (main: List Block)
+  | mk (funs : List Func)
 
-abbrev Scope := Nat
+
 abbrev FuncSigs := List FuncSig
 abbrev BlockSigs := List BlockSig
 
+/-
 namespace Oblg
 --  @[simp] abbrev spoin
   deriving instance DecidableEq for Oblg
@@ -125,26 +125,80 @@ namespace Oblg
     | exit n => exit n
     | spoin σ _n => σ
     | join σ _n => σ
-  
+  @[simp] abbrev last : Oblg -> Nat
+    | retn n => n
+    | exit n => n
+    | spoin σ _n => σ.last
+    | join σ _n => σ.last
+  @[simp] abbrev sig : Oblg -> List Nat
+    | retn _n => []
+    | exit _n => []
+    | spoin σ n => n :: σ.sig
+    | join σ n => n :: σ.sig
+
+
+  inductive RetnExit | Retn | Exit
+  inductive SpoinJoin | Spoin | Join
+  deriving instance DecidableEq for RetnExit
+  deriving instance DecidableEq for SpoinJoin
+
+  abbrev POblg : Type := (RetnExit × Nat) × List (SpoinJoin × Nat)
+  def POblg_Oblg : POblg -> Oblg
+    | ((.Retn, n), []) => .retn n
+    | ((.Exit, n), []) => .exit n
+    | (ren, (.Spoin, n) :: ρ) => (POblg_Oblg (ren, ρ)).spoin n
+    | (ren, (.Join, n) :: ρ) => (POblg_Oblg (ren, ρ)).join n
+  @[simp] theorem POblg_Oblg_Retn (n : Nat) : POblg_Oblg ((.Retn, n), []) = .retn n := by simp[POblg_Oblg]
+  @[simp] theorem POblg_Oblg_Exit (n : Nat) : POblg_Oblg ((.Exit, n), []) = .exit n := by simp[POblg_Oblg]
+  @[simp] theorem POblg_Oblg_Spoin (ren : RetnExit × Nat) (n : Nat) (ρ : List (SpoinJoin × Nat)) : POblg_Oblg (ren, (.Spoin, n) :: ρ) = (POblg_Oblg (ren, ρ)).spoin n := by simp[POblg_Oblg]
+  @[simp] theorem POblg_Oblg_Join (ren : RetnExit × Nat) (n : Nat) (ρ : List (SpoinJoin × Nat)) : POblg_Oblg (ren, (.Join, n) :: ρ) = (POblg_Oblg (ren, ρ)).join n := by simp[POblg_Oblg]
+
+  @[simp] abbrev Oblg_POblg : Oblg -> POblg
+    | .retn n => ((.Retn, n), [])
+    | .exit n => ((.Exit, n), [])
+    | .spoin σ n => let (ren, ρ) := Oblg_POblg σ
+                    (ren, (.Spoin, n) :: ρ)
+    | .join σ n => let (ren, ρ) := Oblg_POblg σ
+                   (ren, (.Join, n) :: ρ)
+
+  @[simp] theorem POblg_Oblg_POblg : (ρ : POblg) -> Oblg_POblg (POblg_Oblg ρ) = ρ
+    | ((.Retn, n), []) => by simp
+    | ((.Exit, n), []) => by simp
+    | (ren, (.Spoin, n) :: ρ) => by simp[POblg_Oblg_POblg (ren, ρ)]
+    | (ren, (.Join, n) :: ρ) => by simp[POblg_Oblg_POblg (ren, ρ)]
+
+  @[simp] theorem Oblg_POblg_Oblg : (σ : Oblg) -> POblg_Oblg (Oblg_POblg σ) = σ
+    | .retn n => by simp
+    | .exit n => by simp
+    | .spoin σ n => by simp[Oblg_POblg_Oblg σ]
+    | .join σ n => by simp[Oblg_POblg_Oblg σ]
 end Oblg
+-/
 
 namespace BlockSig
-  @[simp] abbrev arity | mk a _σ => a
-  @[simp] abbrev oblg | mk _a σ => σ
-  @[simp] abbrev bind | mk a σ => mk a.succ σ
-  @[simp] abbrev retn | mk a _σ, n => mk a (Oblg.retn n)
-  @[simp] abbrev exit | mk a _σ, n => mk a (Oblg.exit n)
-  @[simp] abbrev spoin | mk a σ, n => mk a (σ.spoin n)
-  @[simp] abbrev join | mk a σ, n => mk a (σ.join n)
-  @[simp] abbrev head | mk _a σ => σ.head
-  @[simp] abbrev tail | mk a σ => mk a σ.tail
-  @[simp] abbrev binds | mk a σ, b => mk (a + b) σ
+  @[simp] abbrev Γ | mk Γ _r _σ => Γ
+  @[simp] abbrev r | mk _Γ r _σ => r
+  @[simp] abbrev σ | mk _Γ _r σ => σ
+  @[simp] abbrev bind | mk Γ r σ => mk Γ.succ r σ
+  -- @[simp] abbrev retn | mk Γ _σ, n => mk Γ (Oblg.retn n)
+  -- @[simp] abbrev exit | mk Γ _σ, n => mk Γ (Oblg.exit n)
+  -- @[simp] abbrev spoin | mk Γ σ, n => mk Γ (σ.spoin n)
+  -- @[simp] abbrev join | mk Γ σ, n => mk Γ (σ.join n)
+  -- @[simp] abbrev head | mk _Γ σ => σ.head
+  -- @[simp] abbrev tail | mk Γ σ => mk Γ σ.tail
+  @[simp] abbrev binds | mk Γ r σ, Γ' => mk (Γ + Γ') r σ
 --  @[simp] abbrev join
 
-  -- @[simp] abbrev spork | mk a σ, s => mk a (SporkSig.spwn σ s)
-  -- @[simp] abbrev spoin | mk a σ => mk a σ.tail
+  @[simp] abbrev spork | mk Γ r σ, s => mk Γ r (s :: σ)
+  @[simp] abbrev spoin | mk Γ r σ => mk Γ r σ.tail
+  @[simp] abbrev spwn | mk Γ _r _σ, n => mk Γ n []
+  -- @[simp] abbrev spoin_unpr | mk Γ r σ => mk Γ r σ.tail
+  -- @[simp] abbrev spoin_prom : (bsig : BlockSig) -> bsig.σ ≠ [] -> BlockSig
+  --   | mk Γ r (s :: σ),
 
   deriving instance DecidableEq for BlockSig
+  -- instance : Inhabited BlockSig := ⟨0, .exit 1⟩
+  instance : Inhabited BlockSig := ⟨0, 1, []⟩
 
   -- @[simp] def add (a b : BlockSig) :=
   --   mk (a.arity + b.arity) (a.sporkNest ++ b.sporkNest)
@@ -184,23 +238,6 @@ namespace Var
     coe := idx
 end Var
 
-namespace Var
-  inductive WF (Γ : Scope) (v : Var) : Prop where
-    | mk : v.idx < Γ -> v.WF Γ
-
-  namespace WF
-    notation (name := wfnotation) Γ:arg " ⊢ " v:arg " WF-var" => WF Γ v
-
-    theorem idx {Γ : Scope} {v : Var} : Γ ⊢ v WF-var -> v.idx < Γ | .mk idx => idx
-
-    instance {Γ : Scope} {v : Var} : Decidable (Γ ⊢ v WF-var) :=
-      decidable_of_iff (v.idx < Γ) ⟨(⟨·⟩), (·.1)⟩
-
-    theorem weakening {Γ Γ'} {v : Var} (wf : Γ ⊢ v WF-var) : (Γ + Γ') ⊢ v WF-var :=
-      .mk (Nat.lt_add_right Γ' wf.idx)
-  end WF
-end Var
-
 namespace Atom
   deriving instance DecidableEq for Atom
 end Atom
@@ -234,10 +271,10 @@ namespace Code
     | ite e bthen belse => ([], ⟨ite e bthen belse, by intros e c; simp⟩)
     | call g args bret => ([], ⟨call g args bret, by intros e c; simp⟩)
     | retn args => ([], ⟨retn args, by intros e c; simp⟩)
-    | spork n bbody bspwn => ([], ⟨spork n bbody bspwn, by intros e c; simp⟩)
+    | spork bbody bspwn => ([], ⟨spork bbody bspwn, by intros e c; simp⟩)
     | spoin bunpr bprom => ([], ⟨spoin bunpr bprom, by intros e c; simp⟩)
-    | join bsync => ([], ⟨join bsync, by intros e c; simp⟩)
-    | exit args => ([], ⟨exit args, by intros e c; simp⟩)
+    -- | join bsync => ([], ⟨join bsync, by intros e c; simp⟩)
+    -- | exit args => ([], ⟨exit args, by intros e c; simp⟩)
 
   @[simp] def merge : List Expr -> Code -> Code
     | [], c => c
@@ -256,17 +293,18 @@ namespace Block
   deriving instance DecidableEq for Block
 
   instance : Inhabited Block where
-    default := mk ⟨0, .retn 0⟩ (.retn [])
+    default := mk ⟨0, 0, []⟩ (.retn [])
+             --mk ⟨0, .retn 0⟩ (.retn [])
 end Block
 
 
 namespace Func
   @[simp] abbrev fsig | mk fsig _blocks => fsig
   @[simp] abbrev blocks | mk _fsig blocks => blocks
-  @[simp] abbrev bsigs : Func -> BlockSigs | mk _fsig blocks => blocks.map (·.bsig)
+  @[simp] abbrev B : Func -> BlockSigs | mk _fsig blocks => blocks.map (·.bsig)
   @[simp] abbrev size | mk _fsig blocks => blocks.length
 
-  @[simp] theorem size_eq_bsigs_length (f : Func) : f.bsigs.length = f.size :=
+  @[simp] theorem size_eq_B_length (f : Func) : f.B.length = f.size :=
     by simp
 
   deriving instance DecidableEq for Func
@@ -279,12 +317,11 @@ namespace Func
 end Func
 
 namespace Program
-  @[simp] abbrev funs | mk funs _main => funs
-  @[simp] abbrev main | mk _funs main => main
+  @[simp] abbrev funs | mk funs => funs
   @[simp] abbrev fsigs : Program -> FuncSigs
-    | mk funs _main => funs.map (·.fsig)
+    | mk funs => funs.map (·.fsig)
   @[simp] abbrev size : Program -> Nat
-    | mk funs _main => funs.length
+    | mk funs => funs.length
 
   @[simp] theorem size_eq_fsigs_length (P : Program) : P.fsigs.length = P.size :=
     by simp
@@ -294,504 +331,3 @@ namespace Program
   instance : GetElem Program FuncIdx Func (λ P f => f < P.size) where
     getElem P f p := P.funs[f]
 end Program
-
-/- ==================== Well-Formedness Rules ==================== -/
-
-namespace Atom
-  inductive WF (Γ : Scope) : Atom -> Prop where
-    | val {v : Val} : (val v).WF Γ
-    | var {v : Var} : Γ ⊢ v WF-var -> (var v).WF Γ
-
-  namespace WF
-    notation (name := wfnotation) Γ:arg " ⊢ " a:arg " WF-atom" => WF Γ a
-
-    instance {Γ : Scope} : (a : Atom) -> Decidable (Γ ⊢ a WF-atom)
-      | .val _v => isTrue val
-      | .var v => decidable_of_iff (Γ ⊢ v WF-var) ⟨var, λ (var v) => v⟩
-
-    theorem vwf {Γ : Scope} {v : Var} : Γ ⊢ (Atom.var v) WF-atom -> Γ ⊢ v WF-var
-      | .var wf => wf
-
-    theorem weakening {Γ Γ'} {a : Atom} : Γ ⊢ a WF-atom -> (Γ + Γ') ⊢ a WF-atom
-      | .val => .val
-      | .var wf => .var wf.weakening
-  end WF
-end Atom
-
-namespace Expr  
-  inductive WF (Γ : Scope) : Expr -> Prop where
-    | nop {a : Atom} : Γ ⊢ a WF-atom -> (nop a).WF Γ
-    | uop {o : Uop} {a : Atom} : Γ ⊢ a WF-atom -> (uop o a).WF Γ
-    | bop {o : Bop} {a b : Atom} : Γ ⊢ a WF-atom -> Γ ⊢ b WF-atom -> (bop o a b).WF Γ
-
-  namespace WF
-    notation (name := wfnotation) Γ:arg " ⊢ " e:arg " WF-expr" => WF Γ e
-
-    instance {Γ : Scope} : (e : Expr) -> Decidable (Γ ⊢ e WF-expr)
-      | .nop a => decidable_of_iff (Γ ⊢ a WF-atom)
-          ⟨nop, λ (nop a) => a⟩
-      | .uop _o a => decidable_of_iff (Γ ⊢ a WF-atom)
-          ⟨uop, λ (uop wf) => wf⟩
-      | .bop _o a b => decidable_of_iff (Γ ⊢ a WF-atom ∧ Γ ⊢ b WF-atom)
-          ⟨And.elim bop, λ (bop a b) => ⟨a, b⟩⟩
-
-    theorem weakening {Γ Γ'} {e : Expr} : Γ ⊢ e WF-expr -> (Γ + Γ') ⊢ e WF-expr
-      | .nop a => .nop a.weakening
-      | .uop a => .uop a.weakening
-      | .bop a b => .bop a.weakening b.weakening
-  end WF
-end Expr
-
-namespace Cont
-  -- a continuation that takes `bsig.arity + rets` args
-  inductive WFRets (bsigs : BlockSigs) (bsig : BlockSig) (rets : Nat) (b : Cont) : Prop where
-    | mk (_ : b.b < bsigs.length)
-         (_ : bsigs[b.b] = ⟨b.args.length + rets, bsig.oblg⟩)
-         (_ : IVec (bsig.arity ⊢ · WF-var) b.args)
-
-  inductive WF (bsigs : BlockSigs) (bsig : BlockSig) (b : Cont) : Prop where
-    | mk (_ : b.b < bsigs.length)
-         (_ : bsigs[b.b] = ⟨b.args.length, bsig.oblg⟩)
-         (_ : IVec (bsig.arity ⊢ · WF-var) b.args)
-
-  namespace WFRets
-    notation (name := notationwf) bsigs:arg " ; " bsig:arg " ⊢ " b:arg " ( " rets:arg " )" " WF-cont" => WFRets bsigs bsig rets b
-  end WFRets
-  namespace WF
-    notation (name := notationwf) bsigs:arg " ; " bsig:arg " ⊢ " b:arg " WF-cont" => WF bsigs bsig b
-  end WF
-
-  namespace WFRets
-    instance {bsigs : BlockSigs} {bsig : BlockSig} {b : Cont} :
-             Coe (bsigs; bsig ⊢ b(0) WF-cont) (bsigs; bsig ⊢ b WF-cont) where
-      coe := λ ⟨bwf, blen, argswf⟩ => ⟨bwf, blen, argswf⟩
-
-    instance wf {bsigs : BlockSigs} {bsig : BlockSig} {rets : Nat} {b : Cont} :
-                Decidable (bsigs; bsig ⊢ b(rets) WF-cont) :=
-      dite (b.b < bsigs.length)
-        (λ t => decidable_of_iff
-                  ((bsigs[b.b] = ⟨b.args.length + rets, bsig.oblg⟩) ∧
-                   IVec (bsig.arity ⊢ · WF-var) b.args)
-                  ⟨λ ⟨p1, p2⟩ => ⟨t, p1, p2⟩,
-                   λ ⟨_, p1, p2⟩ => ⟨p1, p2⟩⟩)
-        (λ f => isFalse (f ∘ (λ ⟨p, _, _⟩ => p)))
-
-    abbrev cast0 {bsigs bsig b} : bsigs; bsig ⊢ b(0) WF-cont -> bsigs; bsig ⊢ b WF-cont
-      | ⟨a, b, c⟩ => ⟨a, b, c⟩
-    theorem blt {bsigs bsig rets b} (wf : bsigs; bsig ⊢ b(rets) WF-cont) :
-                b.b < bsigs.length := wf.1
-    theorem bsig {bsigs bsig rets b} (wf : bsigs; bsig ⊢ b(rets) WF-cont) :
-                 bsigs[b.b]'wf.blt = ⟨b.args.length + rets, bsig.oblg⟩ := wf.2
-    theorem args {bsigs bsig rets b} (wf : bsigs; bsig ⊢ b(rets) WF-cont) :
-                 IVec (bsig.arity ⊢ · WF-var) b.args := wf.3
-
-    theorem weakening_bsigs
-            {bsigs bsigs' bsig ret b} :
-            bsigs; bsig ⊢ b(ret) WF-cont ->
-            (bsigs ++ bsigs'); bsig ⊢ b(ret) WF-cont
-      | mk blt bsigb args =>
-        mk (List.length_append ▸ Nat.lt_add_right bsigs'.length blt)
-           (List.getElem_append_left' blt bsigs' ▸ bsigb)
-           args
-  end WFRets
-
-  namespace WF
-    instance {bsigs : BlockSigs} {bsig : BlockSig} {b : Cont} :
-             Coe (bsigs; bsig ⊢ b WF-cont) (bsigs; bsig ⊢ b(0) WF-cont) where
-      coe := λ ⟨bwf, blen, argswf⟩ => ⟨bwf, blen, argswf⟩
-
-    instance wf {bsigs : BlockSigs} {bsig : BlockSig} {b : Cont} :
-                Decidable (bsigs; bsig ⊢ b WF-cont) :=
-      decidable_of_iff (b.WFRets bsigs bsig 0) ⟨Coe.coe, Coe.coe⟩
-
-    abbrev cast0 {bsigs bsig b} : bsigs; bsig ⊢ b WF-cont -> bsigs; bsig ⊢ b(0) WF-cont
-      | ⟨a, b, c⟩ => ⟨a, b, c⟩
-    theorem blt {bsigs bsig b} (wf : bsigs; bsig ⊢ b WF-cont) :
-                b.b < bsigs.length := wf.1
-    theorem bsig {bsigs bsig b} (wf : bsigs; bsig ⊢ b WF-cont) :
-                 bsigs[b.b]'wf.blt = ⟨b.args.length, bsig.oblg⟩ := wf.2
-    theorem args {bsigs bsig b} (wf : bsigs; bsig ⊢ b WF-cont) :
-                 IVec (bsig.arity ⊢ · WF-var) b.args := wf.3
-
-    theorem weakening_bsigs
-            {bsigs bsigs' bsig b}
-            (wf : bsigs; bsig ⊢ b WF-cont) :
-            (bsigs ++ bsigs'); bsig ⊢ b WF-cont :=
-      wf.cast0.weakening_bsigs.cast0
-  end WF
-
-  theorem WFRets0_iff_WF {bsigs : BlockSigs} {bsig : BlockSig} {b : Cont} :
-                         bsigs; bsig ⊢ b(0) WF-cont ↔ bsigs; bsig ⊢ b WF-cont :=
-    ⟨Coe.coe, Coe.coe⟩
-end Cont
-
-namespace Code
-  --notation e:arg " ;; " c => stmt e c
-
-  inductive WF (fsigs : FuncSigs) (bsigs: BlockSigs) : BlockSig -> Code -> Prop where
-    | stmt
-        {bsig : BlockSig}
-        {e : Expr}
-        {c : Code} :
-        bsig.arity ⊢ e WF-expr ->
-        c.WF fsigs bsigs bsig.bind ->
-        (stmt e c).WF fsigs bsigs bsig
-
-    | goto
-        {bsig : BlockSig}
-        {bnext : Cont} :
-        bsigs; bsig ⊢ bnext WF-cont ->
-        (goto bnext).WF fsigs bsigs bsig
-
-    | ite
-        {bsig : BlockSig}
-        {cond : Atom}
-        {bthen : Cont}
-        {belse : Cont} :
-        bsig.arity ⊢ cond WF-atom ->
-        bsigs; bsig ⊢ bthen WF-cont ->
-        bsigs; bsig ⊢ belse WF-cont ->
-        (ite cond bthen belse).WF fsigs bsigs bsig
-
-    | call
-        {bsig : BlockSig}
-        {f : FuncIdx}
-        {args : List Var}
-        {bret : Cont} :
-        (_ : f < fsigs.length) ->
-        fsigs[f].arity = args.length ->
-        IVec (bsig.arity ⊢ · WF-var) args ->
-        bsigs; bsig ⊢ bret(fsigs[f].ret) WF-cont ->
-        (call f args bret).WF fsigs bsigs bsig
-        
-    | retn
-        {bsig : BlockSig}
-        {args : List Var} :
-        bsig.oblg = .retn args.length ->
-        IVec (bsig.arity ⊢ · WF-var) args ->
-        (retn args).WF fsigs bsigs bsig
-
-    | spork
-        {bsig : BlockSig}
-        {bbody : Cont}
-        {bspwn : Cont}
-        {n : Nat} :
-        bsigs; (bsig.spoin n) ⊢ bbody WF-cont ->
-        bsigs; (bsig.exit n) ⊢ bspwn WF-cont ->
-        (spork n bbody bspwn).WF fsigs bsigs bsig
-
-    | spoin
-        {bsig : BlockSig}
-        {bunpr : Cont}
-        {bprom : Cont} :
-        bsig.oblg.isSpoin ->
-        bsigs; bsig.tail ⊢ bunpr WF-cont ->
-        bsigs; (bsig.tail.join bsig.head) ⊢ bprom WF-cont ->
-        (spoin bunpr bprom).WF fsigs bsigs bsig
-    
-    | join
-        {bsig : BlockSig}
-        {bsync : Cont} :
-        bsig.oblg.isJoin ->
-        bsync.WFRets bsigs bsig.tail bsig.head ->
-        (join bsync).WF fsigs bsigs bsig
-    
-    | exit
-        {bsig : BlockSig}
-        {args : List Var}:
-        bsig.oblg = .exit args.length ->
-        IVec (bsig.arity ⊢ · WF-var) args ->
-        (exit args).WF fsigs bsigs bsig
-
-  namespace WF
-    
-    notation (name := notationwf) fsigs:arg " ; " bsigs:arg " ; " bsig:arg " ⊢ " c:arg " WF-code" => WF fsigs bsigs bsig c
---    notation:min (name := notationwf') fsigs:arg bsigs:arg bsig:arg " ⊢ " c " WF-code" => WF fsigs bsigs bsig c
-
-    instance instDecidable {fsigs bsigs bsig} : (c : Code) ->
-                           Decidable (fsigs; bsigs; bsig ⊢ c WF-code)
-      | .stmt e c =>
-          let _ : Decidable (fsigs; bsigs; bsig.bind ⊢ c WF-code) := instDecidable c;
-          decidable_of_iff (bsig.arity ⊢ e WF-expr ∧
-                            fsigs; bsigs; bsig.bind ⊢ c WF-code)
-            ⟨λ ⟨e, c⟩ => stmt e c, λ | stmt e c => ⟨e, c⟩⟩
-      | .goto bnext =>
-          decidable_of_iff (bsigs; bsig ⊢ bnext WF-cont)
-            ⟨goto, λ | goto wf => wf⟩
-      | .ite cond bthen belse =>
-          decidable_of_iff (bsig.arity ⊢ cond WF-atom ∧
-                            bsigs; bsig ⊢ bthen WF-cont ∧
-                            bsigs; bsig ⊢ belse WF-cont)
-            ⟨λ ⟨a, b, c⟩ => ite a b c, λ | ite a b c => ⟨a, b, c⟩⟩
-      | .call f args bret =>
-          decidable_of_iff (∃ _ : f < fsigs.length,
-                            fsigs[f].arity = args.length ∧
-                            IVec (bsig.arity ⊢ · WF-var) args ∧
-                            bsigs; bsig ⊢ bret(fsigs[f].ret) WF-cont)
-            ⟨λ ⟨a, b, c, d⟩ => call a b c d,
-             λ | call a b c d => ⟨a, b, c, d⟩⟩
-      | .retn args =>
-          decidable_of_iff (bsig.oblg = Oblg.retn args.length ∧
-                            IVec (bsig.arity ⊢ · WF-var) args)
-            ⟨λ ⟨a, b⟩ => retn a b, λ | retn a b => ⟨a, b⟩⟩
-      | .spork n bbody bspwn =>
-          decidable_of_iff (bsigs; (bsig.spoin n) ⊢ bbody WF-cont ∧
-                            bsigs; (bsig.exit n) ⊢ bspwn WF-cont)
-            ⟨λ ⟨a, b⟩ => spork a b, λ | spork a b => ⟨a, b⟩⟩
-      | .spoin bunpr bprom =>
-          decidable_of_iff (bsig.oblg.isSpoin ∧
-                            bsigs; bsig.tail ⊢ bunpr WF-cont ∧
-                            bsigs; (bsig.tail.join bsig.head) ⊢ bprom WF-cont)
-            ⟨λ ⟨a, b, c⟩ => spoin a b c, λ | spoin a b c => ⟨a, b, c⟩⟩
-      | .join bsync =>
-          decidable_of_iff (bsig.oblg.isJoin ∧
-                            bsync.WFRets bsigs bsig.tail bsig.head)
-            ⟨λ ⟨a, b⟩ => join a b, λ | join a b => ⟨a, b⟩⟩
-      | .exit args =>
-          decidable_of_iff (bsig.oblg = .exit args.length ∧
-                            IVec (bsig.arity ⊢ · WF-var) args)
-            ⟨λ ⟨a, b⟩ => exit a b, λ | exit a b => ⟨a, b⟩⟩
-
-    -- Accessor methods
-    theorem stmt_expr {fsigs bsigs bsig e c} : fsigs; bsigs; bsig ⊢ (.stmt e c) WF-code -> bsig.arity ⊢ e WF-expr
-      | stmt ewf _cwf => ewf
-    theorem stmt_code {fsigs bsigs bsig e c} : fsigs; bsigs; bsig ⊢ (.stmt e c) WF-code -> fsigs; bsigs; bsig.bind ⊢ c WF-code
-      | stmt _ewf cwf => cwf
-
-    theorem goto_bnext {fsigs bsigs bsig bnext} :
-                       fsigs; bsigs; bsig ⊢ (.goto bnext) WF-code ->
-                       bsigs; bsig ⊢ bnext WF-cont
-      | goto bnextwf => bnextwf
-
-    theorem ite_cond {fsigs bsigs bsig cond bthen belse} :
-                     fsigs; bsigs; bsig ⊢ (.ite cond bthen belse) WF-code ->
-                     bsig.arity ⊢ cond WF-atom
-      | ite condwf _ _ => condwf
-    theorem ite_bthen {fsigs bsigs bsig cond bthen belse} :
-                      fsigs; bsigs; bsig ⊢ (.ite cond bthen belse) WF-code ->
-                      bsigs; bsig ⊢ bthen WF-cont
-      | ite _ bthenwf _ => bthenwf
-    theorem ite_belse {fsigs bsigs bsig cond bthen belse} :
-                      fsigs; bsigs; bsig ⊢ (.ite cond bthen belse) WF-code ->
-                      bsigs; bsig ⊢ belse WF-cont
-      | ite _ _ belsewf => belsewf
-
-    theorem call_flt {fsigs bsigs bsig f args bret} :
-                     fsigs; bsigs; bsig ⊢ (.call f args bret) WF-code ->
-                     f < fsigs.length
-      | call flt _ _ _ => flt
-    theorem call_arity {fsigs bsigs bsig f args bret} :
-                       (wf : fsigs; bsigs; bsig ⊢ (.call f args bret) WF-code) ->
-                       (fsigs[f]'wf.call_flt).arity = args.length
-      | call _ aritywf _ _ => aritywf
-    theorem call_args {fsigs bsigs bsig f args bret} :
-                      fsigs; bsigs; bsig ⊢ (.call f args bret) WF-code ->
-                      IVec (bsig.arity ⊢ · WF-var) args
-      | call _ _ argswf _ => argswf
-    theorem call_bret {fsigs bsigs bsig f args bret} :
-                      (wf : fsigs; bsigs; bsig ⊢ (.call f args bret) WF-code) ->
-                      bsigs; bsig ⊢ bret((fsigs[f]'wf.call_flt).ret) WF-cont
-      | call _ _ _ bretwf => bretwf
-
-    theorem retn_oblg {fsigs bsigs bsig args} :
-                      fsigs; bsigs; bsig ⊢ (.retn args) WF-code ->
-                      bsig.oblg = .retn args.length
-      | retn n _ => n
-    theorem retn_args {fsigs bsigs bsig args} :
-                      fsigs; bsigs; bsig ⊢ (.retn args) WF-code ->
-                      IVec (bsig.arity ⊢ · WF-var) args
-      | retn _ a => a
-
-    theorem spork_bbody {fsigs bsigs bsig n bbody bspwn} :
-                        (wf : fsigs; bsigs; bsig ⊢ (.spork n bbody bspwn) WF-code) ->
-                        bsigs; (bsig.spoin n) ⊢ bbody WF-cont
-      | spork bbodywf _ => bbodywf
-
-    theorem spork_bspwn {fsigs bsigs bsig n bbody bspwn} :
-                        (wf : fsigs; bsigs; bsig ⊢ (.spork n bbody bspwn) WF-code) ->
-                        bsigs; (bsig.exit n) ⊢ bspwn WF-cont
-      | spork _ bspwnwf => bspwnwf
-
-    theorem spoin_oblg {fsigs bsigs bsig bunpr bprom} :
-                       fsigs; bsigs; bsig ⊢ (.spoin bunpr bprom) WF-code ->
-                       bsig.oblg.isSpoin
-      | spoin issp _ _ => issp
-    theorem spoin_bunpr {fsigs bsigs bsig bunpr bprom} :
-                        fsigs; bsigs; bsig ⊢ (.spoin bunpr bprom) WF-code ->
-                        bsigs; bsig.tail ⊢ bunpr WF-cont
-      | spoin _ bunprwf _ => bunprwf
-    theorem spoin_bprom {fsigs bsigs bsig bunpr bprom} :
-                        (wf : fsigs; bsigs; bsig ⊢ (.spoin bunpr bprom) WF-code) ->
-                        bsigs; (bsig.tail.join bsig.head) ⊢ bprom WF-cont
-      | spoin _ _ bpromwf => bpromwf
-
-    theorem weakening_bsigs
-            {fsigs bsigs bsigs' bsig c} :
-            fsigs; bsigs; bsig ⊢ c WF-code ->
-            fsigs; (bsigs ++ bsigs'); bsig ⊢ c WF-code
-      | stmt ewf cwf =>
-        stmt ewf cwf.weakening_bsigs
-      | goto bnextwf =>
-        goto bnextwf.weakening_bsigs
-      | ite ewf bthenwf belsewf =>
-        ite ewf bthenwf.weakening_bsigs belsewf.weakening_bsigs
-      | call flt aritywf argswf bretwf =>
-        call flt aritywf argswf bretwf.weakening_bsigs
-      | retn oblg argswf =>
-        retn oblg argswf
-      | spork bbodywf bspwnwf =>
-        spork bbodywf.weakening_bsigs bspwnwf.weakening_bsigs
-      | spoin snwf bunprwf bpromwf =>
-        spoin snwf bunprwf.weakening_bsigs bpromwf.weakening_bsigs
-      | join oblg bsyncwf =>
-        join oblg bsyncwf.weakening_bsigs
-      | exit oblg argswf =>
-        exit oblg argswf
-
-    theorem merge_wf {fsigs bsigs bsig} :
-            {e : List Expr} -> {c : Code} ->
-            (∀ i : Fin e.length, (bsig.arity + i) ⊢ e[i] WF-expr) ->
-            fsigs; bsigs; (bsig.binds e.length) ⊢ c WF-code ->
-            fsigs; bsigs; bsig ⊢ (c.merge e) WF-code
-      | [], c, ewf, cwf => by simpa using cwf
-      | e :: es, c, ewf, cwf =>
-        .stmt (ewf ⟨0, by simp⟩)
-          (merge_wf (bsig := bsig.bind) (e := es)
-            (λ i => let ewf' := ewf ⟨i.1 + 1, by simp⟩
-                    by simp[← Nat.add_assoc bsig.1 1 i.1] at ewf'
-                       simp
-                       rw[Nat.add_assoc, Nat.add_comm 1 i.1]
-                       exact ewf')
-            (match bsig with
-              | .mk arity sn => by
-                simp
-                simp at cwf
-                rw[Nat.add_comm es.length 1,
-                   ← Nat.add_assoc] at cwf
-                exact cwf))
-
-    theorem split_wf {fsigs bsigs bsig} {c : Code} (cwf : fsigs; bsigs; bsig ⊢ c WF-code) :
-            (∀ i : Fin c.split.1.length, (bsig.arity + i) ⊢ c.split.1[i] WF-expr)
-              ∧ fsigs; bsigs; (bsig.binds c.split.1.length) ⊢ c.split.2.1 WF-code := by
-      cases c <;> try (exact And.intro (λ i => nomatch i) (by simpa using cwf))
-      · case stmt e c =>
-        let p := @split_wf fsigs bsigs bsig.bind c cwf.stmt_code
-        apply And.intro
-        · exact (λ | ⟨0, l⟩ => cwf.stmt_expr
-                   | ⟨i + 1, l⟩ =>
-                     by simpa[Nat.add_assoc, Nat.add_comm 1 i]
-                        using p.1 ⟨i, by simpa using l⟩)
-        · (match h : bsig with
-             | .mk arity sn =>
-               simpa[h, Nat.add_assoc, Nat.add_comm 1]
-               using p.2)
-  end WF
-end Code
-
-namespace Block
-  inductive WF (fsigs bsigs) (b : Block) : Prop where
-    | mk (c : b.code.WF fsigs bsigs b.bsig)
-
-  namespace WF
-    notation (name := notationwf) fsigs:arg " ; " bsigs:arg " ⊢ " b:arg " WF-block" => WF fsigs bsigs b
-
-    instance (fsigs bsigs) : {b : Block} -> Decidable (fsigs; bsigs ⊢ b WF-block)
-      | .mk bsig code =>
-        decidable_of_iff (fsigs; bsigs; bsig ⊢ code WF-code)
-          ⟨λ a => mk a, λ | mk a => a⟩
-
-    theorem code {fsigs bsigs b} : fsigs; bsigs ⊢ b WF-block ->
-                 fsigs; bsigs; b.bsig ⊢ b.code WF-code
-      | .mk c => c
-
-    theorem weakening_bsigs
-            {fsigs bsigs bsigs' b} :
-            fsigs; bsigs ⊢ b WF-block ->
-            fsigs; (bsigs ++ bsigs') ⊢ b WF-block
-      | mk cwf => mk cwf.weakening_bsigs
-  end WF
-end Block
-
-namespace Blocks
-  inductive WF (fsigs : FuncSigs) (bs: List Block) (bsig: BlockSig) : Prop where
-    | mk (blocks : IVec (fsigs; (bs.map (·.bsig)) ⊢ · WF-block) bs)
-         (head : HeadIs bs (·.bsig) bsig)
-
-  namespace WF
-    notation (name := notationwf) fsigs:arg " ; " bsig:arg " ⊢ " bs:arg " WF-blocks" => WF fsigs bs bsig
-
-    instance wf {fsigs: FuncSigs} {bs: List Block} {bsig: BlockSig}:
-                      Decidable (fsigs; bsig ⊢ bs WF-blocks) :=
-      decidable_of_iff (IVec (fsigs; (bs.map (·.bsig)) ⊢ · WF-block) bs ∧
-                        HeadIs bs (·.bsig) bsig)
-        ⟨λ ⟨a, b⟩ => mk a b, λ | mk a b => ⟨a, b⟩⟩
-
-    theorem blocks {fsigs bs bsig} : fsigs; bsig ⊢ bs WF-blocks -> IVec (fsigs; (bs.map (·.bsig)) ⊢ · WF-block) bs
-      | .mk blocks _head => blocks
-    theorem head {fsigs bs bsig} : fsigs; bsig ⊢ bs WF-blocks -> HeadIs bs (·.bsig) bsig
-      | .mk _blocks head => head
-
-    theorem add_blocks
-            {fsigs bs bs' bsig} :
-            fsigs; bsig ⊢ bs WF-blocks ->
-            IVec (fsigs; ((bs ++ bs').map (·.bsig)) ⊢ · WF-block) bs' ->
-            fsigs; bsig ⊢ (bs ++ bs') WF-blocks
-      | .mk blocks head, bs'wf =>
-        .mk (IVec.append (blocks.map
-              (λ b bwf => by simpa using bwf.weakening_bsigs)) bs'wf)
-            ⟨by rw[List.head?_eq_some_head,
-                   List.head_append_left head.nonnil,
-                   ← head.head?eq,
-                   List.head?_eq_head head.nonnil]⟩
-  end WF
-end Blocks
-
-namespace Func
-  -- inductive WF (fsigs : FuncSigs) (f : Func) : Prop where
-  --   | mk (blocks : IVec (·.WF fsigs (f.blocks.map (·.bsig))) f.blocks)
-  --        (head : HeadIs f.blocks (·.bsig) ⟨f.fsig.arity, .retn f.fsig.ret⟩)
-  abbrev WF (fsigs: FuncSigs) (f: Func): Prop :=
-    fsigs; ⟨f.fsig.arity, .retn f.fsig.ret⟩ ⊢ f.blocks WF-blocks
-
-  namespace WF
-    notation (name := notationwf) fsigs:arg " ⊢ " f:arg " WF-func" => WF fsigs f
-    notation (name := notationwf') P:arg " ⊢ " f:arg " WF-func'" => WF (Program.fsigs P) f
-    
-    instance {fsigs : FuncSigs} {f : Func}: Decidable (fsigs ⊢ f WF-func) := Blocks.WF.wf
-
-    theorem blocks {fsigs f} : fsigs ⊢ f WF-func ->
-                   IVec (fsigs; (f.blocks.map (·.bsig)) ⊢ · WF-block) f.blocks
-      := Blocks.WF.blocks
-    theorem head {fsigs f} : fsigs ⊢ f WF-func ->
-                 HeadIs f.blocks (·.bsig) ⟨f.fsig.arity, .retn f.fsig.ret⟩
-      := Blocks.WF.head
-
-    theorem add_blocks
-            {fsigs fsig bs bs'} :
-            fsigs ⊢ (.mk fsig bs) WF-func ->
-            IVec (fsigs; ((bs ++ bs').map (·.bsig)) ⊢ · WF-block) bs' ->
-            fsigs ⊢ (.mk fsig (bs ++ bs')) WF-func :=
-      Blocks.WF.add_blocks
-  end WF
-end Func
-
-namespace Program
-  inductive WF (P : Program): Prop where
-    | mk (funcs : IVec (P ⊢ · WF-func') P.funs)
-         (main: P.fsigs; ⟨0, .exit 1⟩ ⊢ P.main WF-blocks)
-
-  namespace WF
-    notation (name := notationwf) P:arg " WF-program" => WF P
-    
-    instance {P : Program}: Decidable (P WF-program) :=
-      decidable_of_iff (IVec (P.fsigs ⊢ · WF-func) P.funs ∧
-                        P.fsigs; ⟨0, .exit 1⟩ ⊢ P.main WF-blocks)
-          ⟨λ ⟨a, b⟩ => mk a b, λ | mk a b => ⟨a, b⟩⟩
-
-    theorem funcs {P} : P WF-program -> IVec (P.fsigs ⊢ · WF-func) P.funs
-      | .mk funcs _main => funcs
-    theorem main {P} : P WF-program -> P.fsigs; ⟨0, .exit 1⟩ ⊢ P.main WF-blocks
-      | mk _funcs main => main
-  end WF  
-end Program
-
