SporkProofs/WFSemantics.lean
@@ -1,0 +1,434 @@
+import SporkProofs.Syntax
+import SporkProofs.WFSyntax
+import SporkProofs.Semantics
+import SporkProofs.IVec
+import SporkProofs.HeadIs
+
+namespace StackFrameCode
+  inductive WF (fsigs B bsig ret) : StackFrameCode -> Prop
+    | code {c} : c.WF fsigs B bsig -> (code c).WF fsigs B bsig ret
+    | cont {b} : b.WFRets B bsig ret -> (cont b).WF fsigs B bsig ret
+
+  namespace WF
+    notation (name := notationwf) fsigs:arg " ; " B:arg " ; " bsig:arg " ; " ret:arg " ⊢ " c:arg " WF-sfc" => WF fsigs B bsig ret c
+
+    instance {fsigs B bsig ret} : (c : StackFrameCode) ->
+             Decidable (fsigs; B; bsig; ret ⊢ c WF-sfc)
+      | .code c =>
+        decidable_of_iff (fsigs; B; bsig ⊢ c WF-code)
+          ⟨code, λ (code p) => p⟩
+      | .cont b =>
+        decidable_of_iff (B; bsig ⊢ b(ret) WF-cont)
+          ⟨cont, λ (cont p) => p⟩
+
+    theorem c {fsigs B bsig ret c} :
+             fsigs; B; bsig; ret ⊢ (.code c) WF-sfc ->
+             fsigs; B; bsig ⊢ c WF-code
+      | code c => c
+
+    theorem b {fsigs B bsig b ret} :
+             fsigs; B; bsig; ret ⊢ (.cont b) WF-sfc ->
+             B; bsig ⊢ b(ret) WF-cont
+      | cont b => b
+  end WF
+end StackFrameCode
+
+/-
+  inductive WF (B : BlockSigs) (bsig : BlockSig) (b : Cont) : Prop where
+    | mk (_ : b.b < B.length)
+         (_ : B[b.b] = ⟨b.args.length, bsig.σ⟩)
+         (_ : IVec (bsig.Γ ⊢ · WF-var) b.args)
+-/
+
+namespace SpawnBlock
+  inductive WF (B : BlockSigs) (bspwn : SpawnBlock) : Prop where
+    | mk (_ : bspwn.b < B.length)
+         (_ : B[bspwn.b].Γ = bspwn.args.length)
+         (_ : B[bspwn.b].σ.isExit)
+
+  namespace WF
+    notation (name := notationwf) B:arg " ⊢ " bspwn:arg " WF-spawn" => WF B bspwn
+    
+    instance {B: BlockSigs} (bspwn: SpawnBlock): Decidable (B ⊢ bspwn WF-spawn) :=
+      decidable_of_iff (∃ _ :bspwn.b < B.length,
+                        B[bspwn.b].Γ = bspwn.args.length ∧
+                        B[bspwn.b].σ.isExit)
+        ⟨λ ⟨a, b, c⟩ => .mk a b c, λ | .mk a b c => ⟨a, b, c⟩⟩
+
+    theorem b {B bspwn}: B ⊢ bspwn WF-spawn -> bspwn.b < B.length
+      | mk b _args _ex => b
+    theorem args {B bspwn}: (wf : B ⊢ bspwn WF-spawn) -> (B[bspwn.b]'(b wf)).Γ = bspwn.args.length
+      | mk _b args _ex => args
+    theorem isExit {B bspwn}: (wf : B ⊢ bspwn WF-spawn) -> (B[bspwn.b]'(b wf)).σ.isExit
+      | mk _b _args ex => ex
+    abbrev getExit {B bspwn} (wf: B ⊢ bspwn WF-spawn): Nat :=
+      (B[bspwn.b]'(b wf)).σ.getExit wf.isExit
+  end WF
+end SpawnBlock
+
+
+namespace SpawnDeque
+  abbrev SpawnOrder (canProm : Bool) (prom : List SpawnBlock) : Prop :=
+    prom = if canProm then prom else []
+
+  namespace SpawnOrder
+    theorem of_nil {canProm : Bool} : SpawnOrder canProm [] :=
+      by cases canProm <;> rfl
+    theorem prom_canProm_true : (canProm : Bool) -> {bspwn : SpawnBlock} -> {prom : List SpawnBlock} ->
+                                SpawnOrder canProm (bspwn :: prom) -> canProm = true
+      | true, _gret, _prom, _so => rfl
+  end SpawnOrder
+
+  inductive WF (B: BlockSigs) (canProm: Bool) (ρ: SpawnDeque) : Prop
+    | mk (_ : IVec (B ⊢ · WF-spawn) ρ.unpr) (_: SpawnOrder canProm ρ.prom)
+
+  namespace WF
+    notation (name := notationwf) B:arg " ; " canProm:arg " ⊢ " ρ:arg " WF-deque" => WF B canProm ρ
+  
+    instance {B canProm} : (ρ : SpawnDeque) -> Decidable (B; canProm ⊢ ρ WF-deque)
+      | .mk u p => decidable_of_iff
+          (IVec (B ⊢ · WF-spawn) u ∧ SpawnOrder canProm p)
+          ⟨λ ⟨a, b⟩ => ⟨a, b⟩, λ ⟨a, b⟩ => ⟨a, b⟩⟩
+    
+    theorem unpr {fsigs canProm} {ρ : SpawnDeque} : fsigs; canProm ⊢ ρ WF-deque -> IVec (fsigs ⊢ · WF-spawn) ρ.unpr | mk u _p => u
+    theorem prom {fsigs canProm} {ρ : SpawnDeque} : fsigs; canProm ⊢ ρ WF-deque -> SpawnOrder canProm ρ.prom | mk _u p => p
+
+    theorem castCanProm {fsigs ρ} : {canProm : Bool} -> (canProm' : Bool) -> canProm ≤ canProm' -> fsigs; canProm ⊢ ρ WF-deque -> fsigs; canProm' ⊢ ρ WF-deque
+      | false, false, _, .mk MatchesOblg p => .mk MatchesOblg p
+      | true, true, _, .mk u p => .mk u p
+      | false, true, _, .mk u _p => .mk u rfl
+
+    theorem promote {fsigs u p bspwn} (wf : fsigs; true ⊢ ⟨bspwn :: u, p⟩ WF-deque) :
+                    fsigs; true ⊢ ⟨u, bspwn :: p⟩ WF-deque :=
+      ⟨wf.unpr.tail, rfl⟩
+
+    theorem empty {fsigs canProm} : fsigs; canProm ⊢ ∅ WF-deque :=
+      ⟨.nil, .of_nil⟩
+  end WF
+
+  -- abbrev oblg : (ex: Nat) -> SpawnDeque -> Oblg
+  --   | ex,
+  -- inductive MatchesOblg (B : List BlockSig) : SpawnDeque -> Oblg -> Prop where
+  --   | join_π (bspwn : SpawnBlock) (π : List SpawnBlock) (σ : Oblg) :
+  --            MatchesOblg B ⟨[], π⟩ σ ->
+  --            MatchesOblg B ⟨[], bspwn :: π⟩ (σ.join B[bspwn.b]!.σ.last)
+  --   | spoin_π (bspwn : SpawnBlock) (π : List SpawnBlock) (σ : Oblg) :
+  --             MatchesOblg B ⟨[], π⟩ σ ->
+  --             MatchesOblg B ⟨[], bspwn :: π⟩ (σ.spoin B[bspwn.b]!.σ.last)
+  --   | spoin_υ (bspwn : SpawnBlock) (υ π : List SpawnBlock) (σ : Oblg) :
+  --             MatchesOblg B ⟨υ, π⟩ σ ->
+  --             MatchesOblg B ⟨υ.concat bspwn, π⟩ (σ.spoin B[bspwn.b]!.σ.last)
+  --   | retn (n : Nat) : MatchesOblg B ⟨[], []⟩ (.retn n)
+  --   | exit (n : Nat) : MatchesOblg B ⟨[], []⟩ (.exit n)
+
+  -- namespace MatchesOblg
+  --   instance decide_matches_oblg {B: List BlockSig} :
+  --                                (ρ : SpawnDeque) -> (σ : Oblg) ->
+  --                                Decidable (MatchesOblg B ρ σ)
+  --     | ⟨[], bspwn :: π⟩, .join σ n => sorry
+  --     | ⟨[], bspwn :: π⟩, .spoin σ n => sorry
+  --     | ⟨b_end :: υ, π⟩, .spoin σ n => sorry
+  --     | ⟨[], []⟩, .retn n => isTrue sorry
+  --     | ⟨[], []⟩, .exit n => isTrue sorry
+  --     | ⟨_ :: _, _⟩, .retn n => isFalse sorry
+  --     | ⟨_, _ :: _⟩, .retn n => isFalse sorry
+  --     | ⟨_ :: _, _⟩, .exit n => isFalse sorry
+  --     | ⟨_, _ :: _⟩, .exit n => isFalse sorry
+  --     | ⟨_ :: _, _⟩, .join σ n => isFalse sorry
+  --     | ⟨[], []⟩, .join σ n => isFalse sorry
+  --     | ⟨[], []⟩, .spoin σ n => isFalse
+  -- end MatchesOblg
+end SpawnDeque
+
+namespace StackFrame
+  inductive WF (P : Program) (curr : Option Nat) (K : CallStack) (σ : Oblg) :
+               StackFrame -> Prop where
+    | mk {f ρ X c} :
+         (_ : f < P.size) ->
+         (σ : Oblg) ->
+         ρ.sig P[f].B = σ.sig ->
+         ρ.WF P[f].B K.allPromoted ->
+         (if curr.isNone then c.isCode else c.isCont) = true ->
+         c.WF P P[f].B ⟨X.length, σ⟩
+                (curr.elim P[f].fsig.ret id) ->
+         (mk f ρ X c).WF P curr K
+
+  namespace WF
+    instance {P curr K} : (k : StackFrame) -> Decidable (k.WF P curr K)
+      | .mk f ρ X c =>
+        decidable_of_iff (∃ _ : f < P.size,
+                          
+                          ρ.WF P[f].B K.allPromoted ∧
+                          (if curr.isNone then c.isCode else c.isCont) = true ∧
+                          c.WF P.fsigs P[f].B ⟨X.length, ρ.sig⟩
+                            (curr.elim P[f].fsig.ret id))
+          ⟨λ ⟨a, b, c, d⟩ => ⟨a, b, c, d⟩, λ ⟨a, b, c, d⟩ => ⟨a, b, c, d⟩⟩
+
+    theorem flt {P curr canProm} : {k : StackFrame} ->
+                k.WF P curr canProm -> k.f < P.size
+      | .mk _f _ρ _X _c, mk flt _ρwf _cwf _cb => flt
+  end WF
+
+  @[simp] def func {P curr canProm} (k : StackFrame) (kwf : k.WF P curr canProm) : Func :=
+    P[k.f]'kwf.flt
+
+  namespace WF
+
+    theorem ρwf {P curr canProm} : {k : StackFrame} ->
+                k.WF P curr canProm -> k.ρ.WF P.fsigs canProm
+      | .mk _f _ρ _X _c, mk _flt ρwf _cwf _cb => ρwf
+    theorem cwf {P curr canProm} : {k : StackFrame} -> (kwf : k.WF P curr canProm) ->
+                k.c.WF P.fsigs (k.func kwf).B k.bsig
+                         (curr.elim (k.func kwf).fsig.ret id)
+      | .mk _f _ρ _X _c, mk _flt _ρwf _cb cwf => cwf
+    theorem cwf' {P curr canProm} : {k : StackFrame} -> (kwf : k.WF P curr canProm) ->
+                 k.c.WF P.fsigs P[k.f]!.B k.bsig
+                          (curr.elim P[k.f]!.fsig.ret id)
+      | .mk f _ρ _X _c, mk flt _ρwf _cb cwf =>
+        getElem!_pos P f flt ▸ cwf
+    theorem cwf'' {P curr canProm} : {k : StackFrame} -> (kwf : k.WF P curr canProm) ->
+                  let flt : k.f < P.size := kwf.flt
+                  k.c.WF P.fsigs P[k.f].B k.bsig
+                           (curr.elim P[k.f].fsig.ret id)
+      | .mk _f _ρ _X _c, mk _flt _ρwf _cb cwf => cwf
+    theorem cb {P curr canProm} : {k : StackFrame} -> (kwf : k.WF P curr canProm) ->
+               (if curr.isNone then k.c.isCode else k.c.isCont) = true
+      | .mk _f _ρ _X _c, mk _flt _ρwf cb _cwf => cb
+    theorem isCode {P canProm} : {k : StackFrame} ->
+                   (kwf : k.WF P none canProm) -> k.c.isCode := cb
+    theorem isCont {P canProm ret} : {k : StackFrame} ->
+                   (kwf : k.WF P (some ret) canProm) -> k.c.isCont := cb
+
+    theorem castCanProm {P curr canProm} : {k : StackFrame} ->
+                        (canProm' : Bool) -> canProm ≤ canProm' ->
+                        (kwf : k.WF P curr canProm) -> k.WF P curr canProm'
+      | .mk _f _ρ _X _c, canProm', l, .mk flt ρwf cwf cb =>
+        .mk flt (ρwf.castCanProm canProm' l) cwf cb
+
+    theorem entry
+        {P} (Pwf : P.WF) {f canProm} {X : List Val}
+        (p : f < P.size)
+        (sigwf : P[f].fsig.arity = X.length) :
+        WF P none canProm ⟨f, ∅, X, .codeEntry P f⟩ :=
+      let fwf := Pwf.1.get ⟨f, p⟩
+      let c' : Code.WF P.fsigs P[f].B P[f].fsig.ret
+                ⟨X.length, []⟩ P[f]!.blocks.head!.code :=
+        sigwf ▸
+        Eq.symm (getElem!_pos P f p) ▸
+        fwf.2.headeq ▸
+        fwf.2.head!eq ▸
+        (fwf.1.head fwf.2.nonnil).1
+      ⟨p, SpawnDeque.WF.empty, rfl, .code c'⟩
+
+    theorem goto_rets
+        {P} (Pwf : P.WF) {f canProm ρ} {X Y : ValMap} {bnext} {y : List Var}
+        (p : f < P.size)
+        (ρwf : ρ.WF P.fsigs canProm)
+        (bnext_wf : bnext.WFRets P[f].B ⟨X.length, ρ.sig⟩ y.length)
+        (y_wf : IVec (·.WF Y.length) y) :
+        StackFrame.WF P none canProm
+          ⟨f, ρ, X[bnext.args]! ++ Y[y]!, .codeOf P f bnext⟩ :=
+      let ⟨bwf, sigwf, x_wf⟩ := bnext_wf
+      let bwf' : bnext.b < P[f].size :=
+        by simp; exact (List.length_map Block.bsig ▸ bwf)
+      let xlen : bnext.args.length = X[bnext.args].length :=
+        x_wf.map_length (λ x xwf => X[x])
+      let ylen : y.length = Y[y].length :=
+        y_wf.map_length (λ y ywf => Y[y])
+      let code_wf : P[f]![bnext.b]!.code.WF
+                      P.fsigs P[f].B P[f].fsig.ret
+                      ⟨(X[bnext.args]! ++ Y[y]!).length, ρ.sig⟩ := by
+        rw[codeOfGetElem p bwf',
+           argsOfGetElem x_wf,
+           argsOfGetElem y_wf,
+           List.length_append,
+           ← xlen, ← ylen]
+        simp at sigwf
+        simp
+        rw[← sigwf];
+        exact ((Pwf.1.get ⟨f, p⟩).1.get ⟨bnext.b, bwf'⟩).1
+      ⟨p, ρwf, rfl, .code code_wf⟩
+  
+    theorem goto
+        {P} (Pwf : P.WF) {f canProm ρ} {X : ValMap} {bnext}
+        (p : f < P.size)
+        (ρwf : ρ.WF P.fsigs canProm)
+        (bnext_wf : bnext.WF P[f].B ⟨X.length, ρ.sig⟩) :
+        StackFrame.WF P none canProm ⟨f, ρ, X[bnext.args]!, .codeOf P f bnext⟩ :=
+      List.append_nil X[bnext.args]! ▸
+      goto_rets Pwf (Y := []) (y := []) p ρwf bnext_wf.cast0 .nil
+  
+    theorem goto_entry
+        {P} (Pwf : P.WF) {f canProm} {X : ValMap} {x : List Var}
+        (p : f < P.size)
+        (xwf : IVec (·.WF X.length) x)
+        (sigwf : P[f].fsig.arity = x.length) :
+        StackFrame.WF P none canProm ⟨f, ∅, X[x]!, .codeEntry P f⟩ :=
+      entry Pwf p (argsOfGetElem xwf ▸
+                    xwf.map_length (λ x xwf => X[x]) ▸
+                    sigwf)
+  
+  end WF
+end StackFrame
+
+
+namespace CallStack
+  /--
+  (Potentially partial) call stack.
+  When `get` is omitted (`none`), this must be a full call
+  stack, where the current frame has `code` rather than `cont`
+  When `get` is `some n`, it is a partial call stack awaiting
+  a return of `n` args from the following stack frame
+  -/
+  inductive WF (P : Program) : (get : Option Nat := none) -> CallStack -> Prop where
+    | nil {gets} : nil.WF P (some gets)
+    | cons {K k gets} :
+           (kwf : k.WF P gets K.allPromoted) ->
+           K.WF P (k.func kwf).fsig.ret ->
+           (K ⬝ k).WF P gets
+
+  namespace WF
+    notation (name := callstackwfcons) t " ⬝wf " h:arg => WF.cons h t
+
+    instance instDecidable {P} : {gets : Option Nat} -> (K : CallStack) ->
+                           Decidable (K.WF P gets)
+      | some gets, .nil => isTrue WF.nil
+      | none, .nil => isFalse (by cases ·)
+      | gets, K ⬝ k =>
+        dite (k.WF P gets K.allPromoted)
+          (λ kwf => let Kwfdec : Decidable (K.WF P (some (k.func kwf).fsig.ret)) :=
+                      instDecidable K
+                    decidable_of_iff (K.WF P (some (k.func kwf).fsig.ret))
+                      ⟨cons kwf, λ | cons _kwf' Kwf => Kwf⟩)
+          (isFalse ∘ λ | kₙwf, cons kwf _Kwf => kₙwf kwf)
+
+    theorem nonnil {P} {K : CallStack} (Kwf : K.WF P none) : K ≠ CallStack.nil :=
+      by cases Kwf <;> simp
+    theorem head' {P gets} :
+                  {K : CallStack} ->
+                  (nn : K ≠ CallStack.nil) ->
+                  K.WF P gets ->
+                  (K.head nn).WF P gets K.tail.allPromoted
+      | _K ⬝ _k, _nn, _Kwf ⬝wf kwf => kwf
+    theorem tail' {P gets} :
+                  {K : CallStack} ->
+                  (nn : K ≠ CallStack.nil) ->
+                  (Kwf : K.WF P gets) ->
+                  K.tail.WF P (some (P[(K.head nn).f]'(Kwf.head' nn).flt).fsig.ret)
+      | _K ⬝ _k, _nn, Kwf ⬝wf _kwf => Kwf
+
+    theorem head {P gets K k} (Kwf : (K ⬝ k).WF P gets) :
+                 k.WF P gets K.allPromoted :=
+      head' (by simp) Kwf
+
+    theorem tail {P gets K k} (Kwf : (K ⬝ k).WF P gets) :
+                  K.WF P (some (P[k.f]'Kwf.head.flt).fsig.ret) :=
+      tail' (by simp) Kwf
+  end WF
+
+  @[simp] def retjoin?! {P get} : (K : CallStack) -> K.WF P get -> Option Nat
+    | .nil, _wf => none
+    | .nil ⬝ k, wf => some (k.func wf.head).fsig.ret
+    | K ⬝ _k, wf => K.retjoin?! wf.tail
+  
+  theorem retjoin_eq_retjoin?! {P get} : {K : CallStack} -> (wf : K.WF P get) ->
+          (if K = .nil then none else some (K.retjoin P)) = K.retjoin?! wf
+    | .nil, _wf =>
+      rfl
+    | .nil ⬝ k, (_ ⬝wf kwf) =>
+      congrArg (α := Func) (λ x => some x.fsig.ret) (getElem!_pos P k.f kwf.flt)
+    | K ⬝ k ⬝ _k', wf =>
+      retjoin_eq_retjoin?! (K := K ⬝ k) wf.tail
+
+  namespace WF
+    theorem append {P} : {K K' : CallStack} -> {gets : Option Nat} ->
+                   K.WF P (some (K'.retjoin P)) -> K'.WF P gets ->
+                   (gets.isNone ∨ K' ≠ .nil) -> K.allPromoted -> (K ++ K').WF P gets
+      | K, .nil ⬝ k, gets, Kwf, K'wf@(.nil ⬝wf kwf), _, kprom =>
+        by simp; exact
+          (Option.some_inj.mp (retjoin_eq_retjoin?! K'wf) ▸ Kwf) ⬝wf (kprom ▸ kwf)
+      | K, K' ⬝ k' ⬝ k, gets, Kwf, K'wf ⬝wf kwf, p, kprom =>
+        let kprom' := allPromoted_iff_nil.mp kprom
+        let kp : (K' ⬝ k').unpr = (K ++ (K' ⬝ k')).unpr :=
+          by simp; rw[kprom']
+        (append Kwf K'wf (Or.inr (by simp)) kprom) ⬝wf
+          (by simp at kwf; simp; rw[kprom']; exact kwf)
+
+    theorem unappend {P} : {get : Option Nat} -> {K K' : CallStack} ->
+                     (K ++ K').WF P get -> (K' ≠ .nil) -> K.allPromoted ->
+                     K.WF P (some (K'.retjoin P)) ∧ K'.WF P get
+      | get, K, .nil ⬝ k, wf, _, kprom =>
+        let wf' : (K ⬝ k).WF P get :=
+          by rw[@append_cons K .nil k] at wf; exact wf
+        let k_wf : k.WF P get true :=
+          kprom ▸ wf'.head
+        ⟨by simp only[retjoin]
+            rw[getElem!_pos P k.f k_wf.flt]
+            exact wf'.tail,
+         .nil ⬝wf k_wf⟩
+      | get, K, (K' ⬝ k') ⬝ k, wf, _, kprom =>
+        let ⟨Kwf, K'wf⟩ := unappend wf.tail (by simp) kprom
+        let kprom' := allPromoted_iff_nil.mp kprom
+        let kp : [] ++ (K' ⬝ k').unpr = K.unpr ++ (K' ⬝ k').unpr :=
+          kprom'.symm ▸ rfl
+        let k'wf : k.WF P get (K' ⬝ k').allPromoted := by
+          show k.WF P get ((K' ⬝ k').unpr = [])
+          rw[← List.nil_append (K' ⬝ k').unpr, kp, ← append_unpr]
+          exact wf.head
+        ⟨Kwf, K'wf ⬝wf k'wf⟩
+  end WF
+end CallStack
+
+namespace ThreadTree
+  inductive WF (P : Program) : ThreadTree -> Prop where
+    | thread {K} :
+           (Kwf : K.WF P none) ->
+           (thread K).WF P
+    | node {Rp Rc} :
+          (Rpwf : Rp.WF P) ->
+          (Rcwf : Rc.WF P) ->
+          (Rp.prom.head? = some (Rc.retjoin P)) ->
+          (Rc.prom = []) ->
+          (node Rp Rc).WF P
+
+  namespace WF
+    theorem get {P K} : (ThreadTree.thread K).WF P -> K.WF P
+      | thread Kwf => Kwf
+    theorem child {P Rp Rc} : (ThreadTree.node Rp Rc).WF P -> Rc.WF P
+      | node _Rpwf Rcwf _Rpprom _Rcprom => Rcwf
+    theorem parent {P Rp Rc} : (ThreadTree.node Rp Rc).WF P -> Rp.WF P
+      | node Rpwf _Rcwf _Rprom _Rcprom => Rpwf
+    theorem parent_prom {P Rp Rc} : (ThreadTree.node Rp Rc).WF P ->
+                                 Rp.prom.head? = some (Rc.retjoin P)
+      | node _Rpwf _Rcwf Rpprom _Rcprom => Rpprom
+    theorem child_prom {P Rp Rc} : (ThreadTree.node Rp Rc).WF P -> Rc.prom = []
+      | node _Rpwf _Rcwf _Rpprom Rcprom => Rcprom
+
+    instance instDecidable {P} : (R : ThreadTree) -> Decidable (R.WF P)
+      | .thread K => decidable_of_iff (K.WF P none)
+          ⟨thread, λ | thread Kwf => Kwf⟩
+      | .node Rp Rc =>
+        let _ : Decidable (Rp.WF P) := instDecidable Rp
+        let _ : Decidable (Rc.WF P) := instDecidable Rc
+        decidable_of_iff (Rp.WF P ∧
+                          Rc.WF P ∧
+                          Rp.prom.head? = some (Rc.retjoin P) ∧
+                          Rc.prom = [])
+          ⟨λ ⟨Rwf, Rcwf, Rp, Rcp⟩ => node Rwf Rcwf Rp Rcp,
+           λ | node Rwf Rcwf Rp Rcp => ⟨Rwf, Rcwf, Rp, Rcp⟩⟩
+
+    theorem spawn {P f args ret} (Pwf : P.WF) (fwf : SpawnBlock.WF P.fsigs (.mk f args ret)) :
+                  (spawn P f args).WF P := by
+      apply thread
+      apply (.nil ⬝wf ·)
+      exact StackFrame.WF.entry Pwf
+              (by simp; rw[← List.length_map]; exact fwf.flt)
+              (List.getElem_map (α := Func) (·.fsig) ▸
+               (congrArg (α := FuncSig) (·.arity) fwf.sig).symm)
+
+    theorem init {P} (Pwf : P.WF) : (ThreadTree.init P).WF P :=
+      spawn (ret := 1) Pwf
+        (.mk Pwf.main_lt
+             (Pwf.head.get0eq ▸ (List.getElem_map (l := P.funs) (·.fsig)).symm))
+  end WF
+end ThreadTree
