SporkProofs/WFSyntax.lean
@@ -1,0 +1,524 @@
+import SporkProofs.Syntax
+import SporkProofs.IVec
+import SporkProofs.HeadIs
+
+namespace Var
+  inductive WF (Γ : Scope) (v : Var) : Prop where
+    | mk : v.idx < Γ -> v.WF Γ
+
+  namespace WF
+    notation (name := wfnotation) Γ:arg " ⊢ " v:arg " WF-var" => WF Γ v
+
+    theorem idx {Γ : Scope} {v : Var} : Γ ⊢ v WF-var -> v.idx < Γ | .mk idx => idx
+
+    instance {Γ : Scope} {v : Var} : Decidable (Γ ⊢ v WF-var) :=
+      decidable_of_iff (v.idx < Γ) ⟨(⟨·⟩), (·.1)⟩
+
+    theorem weakening {Γ Γ'} {v : Var} (wf : Γ ⊢ v WF-var) : (Γ + Γ') ⊢ v WF-var :=
+      .mk (Nat.lt_add_right Γ' wf.idx)
+  end WF
+end Var
+
+namespace Atom
+  inductive WF (Γ : Scope) : Atom -> Prop where
+    | val {v : Val} : (val v).WF Γ
+    | var {v : Var} : Γ ⊢ v WF-var -> (var v).WF Γ
+
+  namespace WF
+    notation (name := wfnotation) Γ:arg " ⊢ " a:arg " WF-atom" => WF Γ a
+
+    instance {Γ : Scope} : (a : Atom) -> Decidable (Γ ⊢ a WF-atom)
+      | .val _v => isTrue val
+      | .var v => decidable_of_iff (Γ ⊢ v WF-var) ⟨var, λ (var v) => v⟩
+
+    theorem vwf {Γ : Scope} {v : Var} : Γ ⊢ (Atom.var v) WF-atom -> Γ ⊢ v WF-var
+      | .var wf => wf
+
+    theorem weakening {Γ Γ'} {a : Atom} : Γ ⊢ a WF-atom -> (Γ + Γ') ⊢ a WF-atom
+      | .val => .val
+      | .var wf => .var wf.weakening
+  end WF
+end Atom
+
+namespace Expr  
+  inductive WF (Γ : Scope) : Expr -> Prop where
+    | nop {a : Atom} : Γ ⊢ a WF-atom -> (nop a).WF Γ
+    | uop {o : Uop} {a : Atom} : Γ ⊢ a WF-atom -> (uop o a).WF Γ
+    | bop {o : Bop} {a b : Atom} : Γ ⊢ a WF-atom -> Γ ⊢ b WF-atom -> (bop o a b).WF Γ
+
+  namespace WF
+    notation (name := wfnotation) Γ:arg " ⊢ " e:arg " WF-expr" => WF Γ e
+
+    instance {Γ : Scope} : (e : Expr) -> Decidable (Γ ⊢ e WF-expr)
+      | .nop a => decidable_of_iff (Γ ⊢ a WF-atom)
+          ⟨nop, λ (nop a) => a⟩
+      | .uop _o a => decidable_of_iff (Γ ⊢ a WF-atom)
+          ⟨uop, λ (uop wf) => wf⟩
+      | .bop _o a b => decidable_of_iff (Γ ⊢ a WF-atom ∧ Γ ⊢ b WF-atom)
+          ⟨And.elim bop, λ (bop a b) => ⟨a, b⟩⟩
+
+    theorem weakening {Γ Γ'} {e : Expr} : Γ ⊢ e WF-expr -> (Γ + Γ') ⊢ e WF-expr
+      | .nop a => .nop a.weakening
+      | .uop a => .uop a.weakening
+      | .bop a b => .bop a.weakening b.weakening
+  end WF
+end Expr
+
+namespace Cont
+  -- a continuation that takes `bsig.arity + rets` args
+  inductive WFRets (B : BlockSigs) (bsig : BlockSig) (rets : Nat) (b : Cont) : Prop where
+    | mk (_ : b.b < B.length)
+         (_ : B[b.b] = ⟨b.args.length + rets, bsig.r, bsig.σ⟩)
+         (_ : IVec (bsig.Γ ⊢ · WF-var) b.args)
+
+  inductive WF (B : BlockSigs) (bsig : BlockSig) (b : Cont) : Prop where
+    | mk (_ : b.b < B.length)
+         (_ : B[b.b] = ⟨b.args.length, bsig.r, bsig.σ⟩)
+         (_ : IVec (bsig.Γ ⊢ · WF-var) b.args)
+
+  namespace WFRets
+    notation (name := notationwf) B:arg " ; " bsig:arg " ⊢ " b:arg " ( " rets " )" " WF-cont" => WFRets B bsig rets b
+  end WFRets
+  namespace WF
+    notation (name := notationwf) B:arg " ; " bsig:arg " ⊢ " b:arg " WF-cont" => WF B bsig b
+  end WF
+
+  namespace WFRets
+    instance {B : BlockSigs} {bsig : BlockSig} {b : Cont} :
+             Coe (B; bsig ⊢ b(0) WF-cont) (B; bsig ⊢ b WF-cont) where
+      coe := λ ⟨bwf, blen, argswf⟩ => ⟨bwf, blen, argswf⟩
+
+    instance wf {B : BlockSigs} {bsig : BlockSig} {rets : Nat} {b : Cont} :
+                Decidable (B; bsig ⊢ b(rets) WF-cont) :=
+      dite (b.b < B.length)
+        (λ t => decidable_of_iff
+                  ((B[b.b] = ⟨b.args.length + rets, bsig.r, bsig.σ⟩) ∧
+                   IVec (bsig.Γ ⊢ · WF-var) b.args)
+                  ⟨λ ⟨p1, p2⟩ => ⟨t, p1, p2⟩,
+                   λ ⟨_, p1, p2⟩ => ⟨p1, p2⟩⟩)
+        (λ f => isFalse (f ∘ (λ ⟨p, _, _⟩ => p)))
+
+    abbrev cast0 {B bsig b} : B; bsig ⊢ b(0) WF-cont -> B; bsig ⊢ b WF-cont
+      | ⟨a, b, c⟩ => ⟨a, b, c⟩
+    theorem blt {B bsig rets b} (wf : B; bsig ⊢ b(rets) WF-cont) :
+                b.b < B.length := wf.1
+    theorem bsig {B bsig rets b} (wf : B; bsig ⊢ b(rets) WF-cont) :
+                 B[b.b]'wf.blt = ⟨b.args.length + rets, bsig.r, bsig.σ⟩ := wf.2
+    theorem args {B bsig rets b} (wf : B; bsig ⊢ b(rets) WF-cont) :
+                 IVec (bsig.Γ ⊢ · WF-var) b.args := wf.3
+
+    theorem weakening_B
+            {B B' bsig ret b} :
+            B; bsig ⊢ b(ret) WF-cont ->
+            (B ++ B'); bsig ⊢ b(ret) WF-cont
+      | mk blt bsigb args =>
+        mk (List.length_append ▸ Nat.lt_add_right B'.length blt)
+           (List.getElem_append_left' blt B' ▸ bsigb)
+           args
+  end WFRets
+
+  namespace WF
+    instance {B : BlockSigs} {bsig : BlockSig} {b : Cont} :
+             Coe (B; bsig ⊢ b WF-cont) (B; bsig ⊢ b(0) WF-cont) where
+      coe := λ ⟨bwf, blen, argswf⟩ => ⟨bwf, blen, argswf⟩
+
+    instance wf {B : BlockSigs} {bsig : BlockSig} {b : Cont} :
+                Decidable (B; bsig ⊢ b WF-cont) :=
+      decidable_of_iff (b.WFRets B bsig 0) ⟨Coe.coe, Coe.coe⟩
+
+    abbrev cast0 {B bsig b} : B; bsig ⊢ b WF-cont -> B; bsig ⊢ b(0) WF-cont
+      | ⟨a, b, c⟩ => ⟨a, b, c⟩
+    theorem blt {B bsig b} (wf : B; bsig ⊢ b WF-cont) :
+                b.b < B.length := wf.1
+    theorem bsig {B bsig b} (wf : B; bsig ⊢ b WF-cont) :
+                 B[b.b]'wf.blt = ⟨b.args.length, bsig.r, bsig.σ⟩ := wf.2
+    theorem args {B bsig b} (wf : B; bsig ⊢ b WF-cont) :
+                 IVec (bsig.Γ ⊢ · WF-var) b.args := wf.3
+
+    theorem weakening_B
+            {B B' bsig b}
+            (wf : B; bsig ⊢ b WF-cont) :
+            (B ++ B'); bsig ⊢ b WF-cont :=
+      wf.cast0.weakening_B.cast0
+  end WF
+
+  theorem WFRets0_iff_WF {B : BlockSigs} {bsig : BlockSig} {b : Cont} :
+                         B; bsig ⊢ b(0) WF-cont ↔ B; bsig ⊢ b WF-cont :=
+    ⟨Coe.coe, Coe.coe⟩
+end Cont
+
+namespace Code
+  --notation e:arg " ;; " c => stmt e c
+
+  inductive WF (P: Program) (B: BlockSigs) : BlockSig -> Code -> Prop where
+    | stmt
+        {bsig : BlockSig}
+        {e : Expr}
+        {c : Code} :
+        bsig.Γ ⊢ e WF-expr ->
+        c.WF P B bsig.bind ->
+        (stmt e c).WF P B bsig
+
+    | goto
+        {bsig : BlockSig}
+        {bnext : Cont} :
+        B; bsig ⊢ bnext WF-cont ->
+        (goto bnext).WF P B bsig
+
+    | ite
+        {bsig : BlockSig}
+        {cond : Atom}
+        {bthen : Cont}
+        {belse : Cont} :
+        bsig.Γ ⊢ cond WF-atom ->
+        B; bsig ⊢ bthen WF-cont ->
+        B; bsig ⊢ belse WF-cont ->
+        (ite cond bthen belse).WF P B bsig
+
+    | call
+        {bsig : BlockSig}
+        {f : FuncIdx}
+        {args : List Var}
+        {bret : Cont} :
+        (_ : f < P.size) ->
+        P[f].fsig.arity = args.length ->
+        IVec (bsig.Γ ⊢ · WF-var) args ->
+        B; bsig ⊢ bret(P[f].fsig.ret) WF-cont ->
+        (call f args bret).WF P B bsig
+        
+    | retn
+        {bsig : BlockSig}
+        {args : List Var} :
+        bsig.r = args.length ->
+        bsig.σ = [] ->
+        IVec (bsig.Γ ⊢ · WF-var) args ->
+        (retn args).WF P B bsig
+
+    | spork
+        {bsig : BlockSig}
+        {bbody : Cont}
+        {bspwn : Cont} :
+        B; (bsig.spork B[bspwn.b]!.r) ⊢ bbody WF-cont ->
+        B; (bsig.spwn B[bspwn.b]!.r) ⊢ bspwn WF-cont ->
+        (spork bbody bspwn).WF P B bsig
+
+    | spoin
+        {bsig : BlockSig}
+        {bunpr : Cont}
+        {bprom : Cont} :
+        (σnn : bsig.σ ≠ []) ->
+        B; bsig.spoin ⊢ bunpr WF-cont ->
+        B; bsig.spoin ⊢ bprom(bsig.σ.head σnn) WF-cont ->
+        (spoin bunpr bprom).WF P B bsig
+    
+    -- | join
+    --     {bsig : BlockSig}
+    --     {bsync : Cont} :
+    --     bsig.σ.isJoin ->
+    --     bsync.WFRets B bsig.tail bsig.head ->
+    --     (join bsync).WF P B bsig
+    
+    -- | exit
+    --     {bsig : BlockSig}
+    --     {args : List Var}:
+    --     bsig.σ = .exit args.length ->
+    --     IVec (bsig.Γ ⊢ · WF-var) args ->
+    --     (exit args).WF P B bsig
+
+  namespace WF
+    
+    notation (name := notationwf) P:arg " ; " B:arg " ; " bsig:arg " ⊢ " c:arg " WF-code" => WF P B bsig c
+
+    instance instDecidable {P B bsig} : (c : Code) ->
+                           Decidable (P; B; bsig ⊢ c WF-code)
+      | .stmt e c =>
+          let _ : Decidable (P; B; bsig.bind ⊢ c WF-code) := instDecidable c;
+          decidable_of_iff (bsig.Γ ⊢ e WF-expr ∧
+                            P; B; bsig.bind ⊢ c WF-code)
+            ⟨λ ⟨e, c⟩ => stmt e c, λ | stmt e c => ⟨e, c⟩⟩
+      | .goto bnext =>
+          decidable_of_iff (B; bsig ⊢ bnext WF-cont)
+            ⟨goto, λ | goto wf => wf⟩
+      | .ite cond bthen belse =>
+          decidable_of_iff (bsig.Γ ⊢ cond WF-atom ∧
+                            B; bsig ⊢ bthen WF-cont ∧
+                            B; bsig ⊢ belse WF-cont)
+            ⟨λ ⟨a, b, c⟩ => ite a b c, λ | ite a b c => ⟨a, b, c⟩⟩
+      | .call f args bret =>
+          decidable_of_iff (∃ _ : f < P.size,
+                            P[f].fsig.arity = args.length ∧
+                            IVec (bsig.Γ ⊢ · WF-var) args ∧
+                            B; bsig ⊢ bret(P[f].fsig.ret) WF-cont)
+            ⟨λ ⟨a, b, c, d⟩ => call a b c d,
+             λ | call a b c d => ⟨a, b, c, d⟩⟩
+      | .retn args =>
+          decidable_of_iff (bsig.r = args.length ∧
+                            bsig.σ = [] ∧
+                            IVec (bsig.Γ ⊢ · WF-var) args)
+            ⟨λ ⟨a, b, c⟩ => retn a b c, λ | retn a b c => ⟨a, b, c⟩⟩
+      | .spork bbody bspwn =>
+          decidable_of_iff (B; (bsig.spork B[bspwn.b]!.r) ⊢ bbody WF-cont ∧
+                            B; (bsig.spwn B[bspwn.b]!.r) ⊢ bspwn WF-cont)
+            ⟨λ ⟨a, b⟩ => spork a b, λ | spork a b => ⟨a, b⟩⟩
+      | .spoin bunpr bprom =>
+          decidable_of_iff (∃ σnn : bsig.σ ≠ [],
+                            B; bsig.spoin ⊢ bunpr WF-cont ∧
+                            B; bsig.spoin ⊢ bprom(bsig.σ.head σnn) WF-cont)
+            ⟨λ ⟨a, b, c⟩ => spoin a b c, λ | spoin a b c => ⟨a, b, c⟩⟩
+      -- | .join bsync =>
+      --     decidable_of_iff (bsig.σ.isJoin ∧
+      --                       bsync.WFRets B bsig.tail bsig.head)
+      --       ⟨λ ⟨a, b⟩ => join a b, λ | join a b => ⟨a, b⟩⟩
+      -- | .exit args =>
+      --     decidable_of_iff (bsig.σ = .exit args.length ∧
+      --                       IVec (bsig.Γ ⊢ · WF-var) args)
+      --       ⟨λ ⟨a, b⟩ => exit a b, λ | exit a b => ⟨a, b⟩⟩
+
+    -- Accessor methods
+    theorem stmt_expr {P B bsig e c} : P; B; bsig ⊢ (.stmt e c) WF-code -> bsig.Γ ⊢ e WF-expr
+      | stmt ewf _cwf => ewf
+    theorem stmt_code {P B bsig e c} : P; B; bsig ⊢ (.stmt e c) WF-code -> P; B; bsig.bind ⊢ c WF-code
+      | stmt _ewf cwf => cwf
+
+    theorem goto_bnext {P B bsig bnext} :
+                       P; B; bsig ⊢ (.goto bnext) WF-code ->
+                       B; bsig ⊢ bnext WF-cont
+      | goto bnextwf => bnextwf
+
+    theorem ite_cond {P B bsig cond bthen belse} :
+                     P; B; bsig ⊢ (.ite cond bthen belse) WF-code ->
+                     bsig.Γ ⊢ cond WF-atom
+      | ite condwf _ _ => condwf
+    theorem ite_bthen {P B bsig cond bthen belse} :
+                      P; B; bsig ⊢ (.ite cond bthen belse) WF-code ->
+                      B; bsig ⊢ bthen WF-cont
+      | ite _ bthenwf _ => bthenwf
+    theorem ite_belse {P B bsig cond bthen belse} :
+                      P; B; bsig ⊢ (.ite cond bthen belse) WF-code ->
+                      B; bsig ⊢ belse WF-cont
+      | ite _ _ belsewf => belsewf
+
+    theorem call_flt {P B bsig f args bret} :
+                     P; B; bsig ⊢ (.call f args bret) WF-code ->
+                     f < P.size
+      | call flt _ _ _ => flt
+    theorem call_arity {P B bsig f args bret} :
+                       (wf : P; B; bsig ⊢ (.call f args bret) WF-code) ->
+                       (P[f]'wf.call_flt).fsig.arity = args.length
+      | call _ aritywf _ _ => aritywf
+    theorem call_args {P B bsig f args bret} :
+                      P; B; bsig ⊢ (.call f args bret) WF-code ->
+                      IVec (bsig.Γ ⊢ · WF-var) args
+      | call _ _ argswf _ => argswf
+    theorem call_bret {P B bsig f args bret} :
+                      (wf : P; B; bsig ⊢ (.call f args bret) WF-code) ->
+                      B; bsig ⊢ bret((P[f]'wf.call_flt).fsig.ret) WF-cont
+      | call _ _ _ bretwf => bretwf
+
+    theorem retn_length {P B bsig args} :
+                        P; B; bsig ⊢ (.retn args) WF-code ->
+                        bsig.r = args.length
+      | retn n _ _ => n
+    theorem retn_oblg {P B bsig args} :
+                      P; B; bsig ⊢ (.retn args) WF-code ->
+                      bsig.σ = []
+      | retn _ σ _ => σ
+    theorem retn_args {P B bsig args} :
+                      P; B; bsig ⊢ (.retn args) WF-code ->
+                      IVec (bsig.Γ ⊢ · WF-var) args
+      | retn _ _ a => a
+
+    theorem spork_bbody {P B bsig bbody bspwn} :
+                        (wf : P; B; bsig ⊢ (.spork bbody bspwn) WF-code) ->
+                        B; (bsig.spork B[bspwn.b]!.r) ⊢ bbody WF-cont
+      | spork bbodywf _ => bbodywf
+
+    theorem spork_bspwn {P B bsig bbody bspwn} :
+                        (wf : P; B; bsig ⊢ (.spork bbody bspwn) WF-code) ->
+                        B; (bsig.spwn B[bspwn.b]!.r) ⊢ bspwn WF-cont
+      | spork _ bspwnwf => bspwnwf
+
+    theorem spoin_oblg {P B bsig bunpr bprom} :
+                       P; B; bsig ⊢ (.spoin bunpr bprom) WF-code ->
+                       bsig.σ ≠ []
+      | spoin issp _ _ => issp
+    theorem spoin_bunpr {P B bsig bunpr bprom} :
+                        P; B; bsig ⊢ (.spoin bunpr bprom) WF-code ->
+                        B; bsig.spoin ⊢ bunpr WF-cont
+      | spoin _ bunprwf _ => bunprwf
+    theorem spoin_bprom {P B bsig bunpr bprom} :
+                        (wf : P; B; bsig ⊢ (.spoin bunpr bprom) WF-code) ->
+                        B; bsig.spoin ⊢ bprom(bsig.σ.head wf.spoin_oblg) WF-cont
+      | spoin _ _ bpromwf => bpromwf
+
+    theorem weakening_B
+            {P B B' bsig c} :
+            P; B; bsig ⊢ c WF-code ->
+            P; (B ++ B'); bsig ⊢ c WF-code
+      | stmt ewf cwf =>
+        stmt ewf cwf.weakening_B
+      | goto bnextwf =>
+        goto bnextwf.weakening_B
+      | ite ewf bthenwf belsewf =>
+        ite ewf bthenwf.weakening_B belsewf.weakening_B
+      | call flt aritywf argswf bretwf =>
+        call flt aritywf argswf bretwf.weakening_B
+      | retn r σ argswf =>
+        retn r σ argswf
+      | spork (bspwn := bspwn) bbodywf bspwnwf =>
+        let h := List.getElem?_append_left bspwnwf.blt (l₂ := B')
+        let spwn := bspwnwf.weakening_B
+        let body := bbodywf.weakening_B
+        spork (by simp; rw[h]; simp at body; exact body)
+              (by simp; rw[h]; simp at spwn; exact spwn)
+      | spoin snwf bunprwf bpromwf =>
+        spoin snwf bunprwf.weakening_B bpromwf.weakening_B
+      -- | join oblg bsyncwf =>
+      --   join oblg bsyncwf.weakening_B
+      -- | exit oblg argswf =>
+      --   exit oblg argswf
+
+    theorem merge_wf {P B bsig} :
+            {e : List Expr} -> {c : Code} ->
+            (∀ i : Fin e.length, (bsig.Γ + i) ⊢ e[i] WF-expr) ->
+            P; B; (bsig.binds e.length) ⊢ c WF-code ->
+            P; B; bsig ⊢ (c.merge e) WF-code
+      | [], c, ewf, cwf => by simpa using cwf
+      | e :: es, c, ewf, cwf =>
+        .stmt (ewf ⟨0, by simp⟩)
+          (merge_wf (bsig := bsig.bind) (e := es)
+            (λ i => let ewf' := ewf ⟨i.1 + 1, by simp⟩
+                    by simp[← Nat.add_assoc bsig.1 1 i.1] at ewf'
+                       simp
+                       rw[Nat.add_assoc, Nat.add_comm 1 i.1]
+                       exact ewf')
+            (match bsig with
+              | .mk Γ r σ => by
+                simp
+                simp at cwf
+                rw[Nat.add_comm es.length 1,
+                   ← Nat.add_assoc] at cwf
+                exact cwf))
+
+    theorem split_wf {P B bsig} {c : Code} (cwf : P; B; bsig ⊢ c WF-code) :
+            (∀ i : Fin c.split.1.length, (bsig.Γ + i) ⊢ c.split.1[i] WF-expr)
+              ∧ P; B; (bsig.binds c.split.1.length) ⊢ c.split.2.1 WF-code := by
+      cases c <;> try (exact And.intro (λ i => nomatch i) (by simpa using cwf))
+      · case stmt e c =>
+        let p := @split_wf P B bsig.bind c cwf.stmt_code
+        apply And.intro
+        · exact (λ | ⟨0, l⟩ => cwf.stmt_expr
+                   | ⟨i + 1, l⟩ =>
+                     by simpa[Nat.add_assoc, Nat.add_comm 1 i]
+                        using p.1 ⟨i, by simpa using l⟩)
+        · (match h : bsig with
+             | .mk Γ r σ =>
+               simpa[h, Nat.add_assoc, Nat.add_comm 1]
+               using p.2)
+  end WF
+end Code
+
+namespace Block
+  inductive WF (P B) (b : Block) : Prop where
+    | mk (c : b.code.WF P B b.bsig)
+
+  namespace WF
+    notation (name := notationwf) P:arg " ; " B:arg " ⊢ " b:arg " WF-block" => WF P B b
+
+    instance (P B) : {b : Block} -> Decidable (P; B ⊢ b WF-block)
+      | .mk bsig code =>
+        decidable_of_iff (P; B; bsig ⊢ code WF-code)
+          ⟨λ a => mk a, λ | mk a => a⟩
+
+    theorem code {P B b} : P; B ⊢ b WF-block ->
+                 P; B; b.bsig ⊢ b.code WF-code
+      | .mk c => c
+
+    theorem weakening_B {P B B' b} : P; B ⊢ b WF-block ->
+                        P; (B ++ B') ⊢ b WF-block
+      | mk cwf => mk cwf.weakening_B
+  end WF
+end Block
+
+namespace Blocks
+  inductive WF (P : Program) (bs: List Block) (bsig: BlockSig) : Prop where
+    | mk (blocks : IVec (P; (bs.map (·.bsig)) ⊢ · WF-block) bs)
+         (head : HeadIs bs (·.bsig) bsig)
+
+  namespace WF
+    notation (name := notationwf) P:arg " ; " bsig:arg " ⊢ " bs:arg " WF-blocks" => WF P bs bsig
+
+    instance wf {P bs bsig}: Decidable (P; bsig ⊢ bs WF-blocks) :=
+      decidable_of_iff (IVec (P; (bs.map (·.bsig)) ⊢ · WF-block) bs ∧
+                        HeadIs bs (·.bsig) bsig)
+        ⟨λ ⟨a, b⟩ => mk a b, λ | mk a b => ⟨a, b⟩⟩
+
+    theorem blocks {P bs bsig} : P; bsig ⊢ bs WF-blocks -> IVec (P; (bs.map (·.bsig)) ⊢ · WF-block) bs
+      | .mk blocks _head => blocks
+    theorem head {P bs bsig} : P; bsig ⊢ bs WF-blocks -> HeadIs bs (·.bsig) bsig
+      | .mk _blocks head => head
+
+    theorem add_blocks
+            {P bs bs' bsig} :
+            P; bsig ⊢ bs WF-blocks ->
+            IVec (P; ((bs ++ bs').map (·.bsig)) ⊢ · WF-block) bs' ->
+            P; bsig ⊢ (bs ++ bs') WF-blocks
+      | .mk blocks head, bs'wf =>
+        .mk (IVec.append (blocks.map
+              (λ b bwf => by simpa using bwf.weakening_B)) bs'wf)
+            ⟨by rw[List.head?_eq_some_head,
+                   List.head_append_left head.nonnil,
+                   ← head.head?eq,
+                   List.head?_eq_head head.nonnil]⟩
+  end WF
+end Blocks
+
+namespace Func
+  -- inductive WF (P : Program) (f : Func) : Prop where
+  --   | mk (blocks : IVec (·.WF P (f.blocks.map (·.bsig))) f.blocks)
+  --        (head : HeadIs f.blocks (·.bsig) ⟨f.fsig.arity, .retn f.fsig.ret⟩)
+  abbrev WF (P: Program) (f: Func): Prop :=
+    P; ⟨f.fsig.arity, f.fsig.ret, []⟩ ⊢ f.blocks WF-blocks
+
+  namespace WF
+    notation (name := notationwf) P:arg " ⊢ " f:arg " WF-func" => WF P f
+    notation (name := notationwf') P:arg " ⊢ " f:arg " WF-func'" => WF (Program.P P) f
+    
+    instance {P f}: Decidable (P ⊢ f WF-func) := Blocks.WF.wf
+
+    theorem blocks {P f} : P ⊢ f WF-func ->
+                   IVec (P; (f.blocks.map (·.bsig)) ⊢ · WF-block) f.blocks
+      := Blocks.WF.blocks
+    theorem head {P f} : P ⊢ f WF-func ->
+                 HeadIs f.blocks (·.bsig) ⟨f.fsig.arity, f.fsig.ret, []⟩
+      := Blocks.WF.head
+
+    theorem add_blocks
+            {P fsig bs bs'} :
+            P ⊢ (.mk fsig bs) WF-func ->
+            IVec (P; ((bs ++ bs').map (·.bsig)) ⊢ · WF-block) bs' ->
+            P ⊢ (.mk fsig (bs ++ bs')) WF-func :=
+      Blocks.WF.add_blocks
+  end WF
+end Func
+
+namespace Program
+  inductive WF (P : Program): Prop where
+    | mk (funcs : IVec (P ⊢ · WF-func) P.funs)
+         (main: HeadIs P.funs (·.fsig) ⟨0, 1⟩)
+
+  namespace WF
+    notation (name := notationwf) P:arg " WF-program" => WF P
+    
+    instance {P : Program}: Decidable (P WF-program) :=
+      decidable_of_iff (IVec (P ⊢ · WF-func) P.funs ∧
+                        HeadIs P.funs (·.fsig) ⟨0, 1⟩)
+          ⟨λ ⟨a, b⟩ => mk a b, λ | mk a b => ⟨a, b⟩⟩
+
+    theorem funcs {P} : P WF-program -> IVec (P ⊢ · WF-func) P.funs
+      | .mk funcs _main => funcs
+    theorem main {P} : P WF-program -> HeadIs P.funs (·.fsig) ⟨0, 1⟩
+      | mk _funcs main => main
+  end WF
+end Program
+
